interp preserves sbisim
for simple enough handlers

theories/Interp/Interp.v
@@ -131,6 +131,673 @@ Proof.
     now constructor; intros.
 Qed.
 
+(** Counter-example showing that interp does not preserve sbisim in the general case. *)
+
+Inductive VoidE : Type -> Type :=
+| voidE : VoidE void.
+
+#[local] Definition t1 := Ret 1 : ctree VoidE nat.
+#[local] Definition t2 := choiceI2 (Ret 1) (x <- trigger voidE;; match x : void with end) : ctree VoidE nat.
+
+Goal t1 ~ t2.
+Proof.
+  unfold t1, t2.
+  rewrite choiceI2_commut.
+  rewrite choiceI2_is_stuck. reflexivity.
+  red. intros. intro. inv_trans.  destruct x.
+Qed.
+
+#[local] Definition h : VoidE ~> ctree VoidE.
+Proof.
+  intros. destruct H. exact (TauV CTree.stuckI).
+Defined.
+
+Example interp_sbsisim_counterexample : ~ (interp h t1 ~ interp h t2).
+Proof.
+  red. intros. unfold t2 in H.
+  playR in H.
+  rewrite unfold_interp. cbn. setoid_rewrite bind_choice.
+  eapply trans_choiceI with (x := Fin.FS Fin.F1).
+  2: { rewrite bind_ret_l. reflexivity. }
+  apply trans_tauI. setoid_rewrite unfold_interp. cbn. rewrite bind_choice. etrans.
+  rewrite unfold_interp in H. unfold t1, h in H. cbn in H. inv_trans.
+Qed.
+
+(** Helper inductive t0_det t t' means that t' is TauI*(t) *)
+
+Inductive t0_det {E X} : relation (ctree E X) :=
+| t0_det_id : forall t t', t ≅ t' -> t0_det t t'
+| t0_det_tau : forall t t' t'',
+    t0_det t t' -> t'' ≅ TauI t -> t0_det t'' t'.
+
+#[global] Instance t0_det_equ : forall {E X}, Proper (equ eq ==> equ eq ==> flip impl) (@t0_det E X).
+Proof.
+  cbn. intros.
+  revert x H. induction H1; intros.
+  - econstructor. now rewrite H0, H1.
+  - eapply t0_det_tau. apply IHt0_det. apply H0. reflexivity. rewrite H2. apply H.
+Qed.
+
+#[global] Instance t0_det_equ' : forall {E X}, Proper (equ eq ==> equ eq ==> impl) (@t0_det E X).
+Proof.
+  cbn. intros. rewrite <- H, <- H0. apply H1.
+Qed.
+
+Lemma t0_det_bind {E X Y} : forall (t t' : ctree E X) (k : X -> ctree E Y),
+  t0_det t t' ->
+  t0_det (t >>= k) (t' >>= k).
+Proof.
+  intros. induction H.
+  - rewrite H. constructor. reflexivity.
+  - rewrite H0. setoid_rewrite bind_tauI. eapply t0_det_tau. apply IHt0_det. reflexivity.
+Qed.
+
+Lemma t0_det_bind_ret_l {E X Y} : forall (t : ctree E X) t' (k : X -> ctree E Y) x,
+  t0_det t (Ret x) ->
+  t0_det (k x) t' ->
+  t0_det (t >>= k) t'.
+Proof.
+  intros. remember (Ret x) as R. revert t' k x HeqR H0. induction H; intros; subst.
+  - subst. rewrite H, bind_ret_l. apply H0.
+  - rewrite H0. setoid_rewrite bind_tauI.
+    eapply t0_det_tau. 2: reflexivity. eapply IHt0_det. reflexivity. apply H1.
+Qed.
+
+Lemma t0_det_bind_ret_l_equ {E X Y} : forall (t : ctree E X) (k : X -> ctree E Y) x,
+  t0_det t (Ret x) ->
+  x <- t;; k x ≅ t;; k x.
+Proof.
+  intros. remember (Ret x) as R. induction H; subst.
+  - rewrite H. rewrite !bind_ret_l. reflexivity.
+  - rewrite H0. rewrite !bind_tauI. apply choice_equ. intro. apply IHt0_det. reflexivity.
+Qed.
+
+Lemma sbisim_t0_det {E X} : forall (t t' : ctree E X), t0_det t t' -> t ~ t'.
+Proof.
+  intros. induction H.
+  - now rewrite H.
+  - rewrite H0. rewrite sb_tauI. apply IHt0_det.
+Qed.
+
+(* is_simple *)
+
+Definition is_simple {E X} (t : ctree E X) :=
+  (forall l t', trans l t t' -> is_val l) \/
+  (forall l t', trans l t t' -> exists r, t0_det t' (Ret r)).
+
+#[global] Instance is_simple_equ : forall {E X},
+  Proper (equ eq ==> iff) (@is_simple E X).
+Proof.
+  cbn. intros. unfold is_simple. setoid_rewrite H. reflexivity.
+Qed.
+
+Lemma is_simple_ret : forall {E X} r, is_simple (Ret r : ctree E X).
+Proof.
+  cbn. red. intros. left. intros. inv_trans. subst. constructor.
+Qed.
+
+Lemma is_simple_tauI_ret : forall {E X} r, is_simple (TauI (Ret r) : ctree E X).
+Proof.
+  cbn. red. intros. left. intros. inv_trans. subst. constructor.
+Qed.
+
+Lemma is_simple_choice : forall {E} n, is_simple (choice false n : ctree E _).
+Proof.
+  cbn. red. intros.
+  left. intros. apply trans_choiceI_inv in H as []. inv_trans. subst. constructor.
+Qed.
+
+Lemma is_simple_choiceI : forall {E X} n (k : fin n -> ctree E X) x,
+  is_simple (ChoiceI n k) -> is_simple (k x).
+Proof.
+  intros. destruct H.
+  - left. intros. eapply H. etrans.
+  - right. intros. eapply H. etrans.
+Qed.
+
+Definition vsimple {E X} (t : ctree E X) :=
+  (exists x, t ≅ Ret x) \/ exists f, t ≅ CTree.trigger f.
+
+(** trans0 *)
+
+Inductive trans0_ {E X} : ctree' E X -> ctree' E X -> Prop :=
+| T0Id : forall t t', t ≅ t' -> trans0_ (observe t) (observe t')
+| T0Choice : forall c k x t, trans0_ (observe (k x)) t -> trans0_ (ChoiceIF c k) t
+.
+
+Definition trans0 {E X} (t t' : ctree E X) := trans0_ (observe t) (observe t').
+
+#[global] Instance trans0_equ_ {E X} :
+  Proper (going (equ eq) ==> going (equ eq) ==> impl) (@trans0_ E X).
+Proof.
+  cbn. intros.
+  revert y y0 H H0. induction H1; intros.
+  - pose (T0Id (go y) (go y0)). cbn in t0. apply t0.
+    rewrite <- H0, <- H1, H. reflexivity.
+  - destruct H. step in H. inv H. invert.
+    econstructor. apply IHtrans0_. constructor.
+    rewrite <- !ctree_eta. apply REL. apply H0.
+Qed.
+
+#[global] Instance trans0_equ_' {E X} :
+  Proper (going (equ eq) ==> going (equ eq) ==> flip impl) (@trans0_ E X).
+Proof.
+  cbn. intros. now rewrite <- H, <- H0 in H1.
+Qed.
+
+#[global] Instance trans0_equ {E X} : Proper (equ eq ==> equ eq ==> iff) (@trans0 E X).
+Proof.
+  unfold trans0. split; intros.
+  - now rewrite <- H, <- H0.
+  - now rewrite H, H0.
+Qed.
+
+Lemma trans0_trans {E X} : forall (t t' : ctree E X),
+  trans0 t t' -> forall l t'', trans l t' t'' -> trans l t t''.
+Proof.
+  intros. red in H. rewrite ctree_eta. rewrite ctree_eta in H0.
+  genobs t ot. genobs t' ot'. clear t Heqot t' Heqot'.
+  induction H.
+  - rewrite H. apply H0.
+  - apply IHtrans0_ in H0. eapply trans_choiceI in H0. apply H0. rewrite <- ctree_eta. reflexivity.
+Qed.
+
+Lemma trans0_fwd : forall {E X} (t : ctree E X) n k (x : fin n),
+  trans0 t (ChoiceI n k) -> trans0 t (k x).
+Proof.
+  intros. red in H. red.
+  genobs t ot. clear t Heqot.
+  remember (observe (ChoiceI n k)) as oc.
+  revert n k x Heqoc. induction H.
+  - intros. rewrite H, Heqoc. eapply T0Choice. constructor. reflexivity.
+  - intros. subst. eapply T0Choice. apply IHtrans0_. reflexivity.
+Qed.
+
+Lemma trans0_interp : forall {E F X} (h : E ~> ctree F) (t t' : ctree E X),
+  trans0 t t' -> trans0 (interp h t) (interp h t').
+Proof.
+  intros. red in H. setoid_rewrite (ctree_eta t). setoid_rewrite (ctree_eta t').
+  genobs t ot. genobs t' ot'. clear t Heqot t' Heqot'.
+  induction H.
+  - constructor. rewrite H. reflexivity.
+  - rewrite unfold_interp. cbn. setoid_rewrite bind_choice.
+    apply T0Choice with (x := x). rewrite bind_ret_l.
+    apply T0Choice with (x := Fin.F1). apply IHtrans0_.
+Qed.
+
+(* productive *)
+
+Inductive productive {E X} : ctree E X -> Prop :=
+| prod_ret {r t} (EQ: t ≅ Ret r) : productive t
+| prod_vis {Y} {e : E Y} {k t} (EQ: t ≅ Vis e k) : productive t
+| prod_tau {n k t} (EQ: t ≅ ChoiceV n k) : productive t.
+
+#[global] Instance productive_equ : forall {E X}, Proper (equ eq ==> impl) (@productive E X).
+Proof.
+  cbn. intros. inv H0; rewrite H in *.
+  - eapply prod_ret; eauto.
+  - eapply prod_vis; eauto.
+  - eapply prod_tau; eauto.
+Qed.
+
+#[global] Instance productive_equ' : forall {E X}, Proper (equ eq ==> flip impl) (@productive E X).
+Proof.
+  cbn. intros. rewrite <- H in H0. apply H0.
+Qed.
+
+Lemma trans_productive {E X} l (t t'' : ctree E X) : trans l t t'' -> exists t',
+  trans0 t t' /\ productive t' /\ trans l t' t''.
+Proof.
+  intros. do 3 red in H.
+  setoid_rewrite (ctree_eta t). setoid_rewrite (ctree_eta t'').
+  genobs t ot. genobs t'' ot''. clear t Heqot t'' Heqot''.
+  induction H; intros.
+  - destruct IHtrans_ as (? & ? & ? & ?).
+    rewrite <- ctree_eta in H0. eapply T0Choice in H0.
+    exists x0. auto.
+  - eexists. split; [| split ].
+    + left. reflexivity.
+    + eapply prod_tau. reflexivity.
+    + rewrite <- H, <- ctree_eta. etrans.
+  - eexists. split; [| split ].
+    + left. reflexivity.
+    + eapply prod_vis. reflexivity.
+    + rewrite <- H, <- ctree_eta. etrans.
+  - eexists. split; [| split ].
+    + left. reflexivity.
+    + eapply prod_ret. reflexivity.
+    + rewrite choice0_always_stuck. etrans.
+Qed.
+
+Lemma interp_productive {E F X} (h : E ~> ctree F) : forall (t : ctree E X),
+  productive (interp h t) -> productive t.
+Proof.
+  intros. inversion H;
+    subst;
+    rewrite unfold_interp in EQ;
+    rewrite (ctree_eta t);
+    destruct (observe t) eqn:?;
+    (try destruct vis);
+    (try step in EQ; inv EQ);
+    try now econstructor.
+Qed.
+
+Lemma productive_trans0 {E X} : forall (t t' : ctree E X),
+  productive t -> trans0 t t' -> t ≅ t'.
+Proof.
+  intros. setoid_rewrite ctree_eta.
+  inversion H; subst; rewrite (ctree_eta t) in EQ; inversion H0; subst.
+  - now rewrite H3.
+  - rewrite <- H1 in EQ. step in EQ. inv EQ.
+  - now rewrite H3.
+  - rewrite <- H1 in EQ. step in EQ. inv EQ.
+  - now rewrite H3.
+  - rewrite <- H1 in EQ. step in EQ. inv EQ.
+Qed.
+
+Lemma trans_val_trans0 {E X} : forall x (t t' : ctree E X),
+  trans (val x) t t' -> trans0 t (Ret x) /\ t' ≅ CTree.stuckI.
+Proof.
+  intros. apply trans_productive in H as (? & ? & ? & ?).
+  inv H0.
+  - rewrite EQ in H, H1. inv_trans. subst. auto.
+  - rewrite EQ in H1. inv_trans.
+  - rewrite EQ in H1. inv_trans.
+Qed.
+
+Lemma trans_tau_trans0 {E X} : forall (t t' : ctree E X),
+  trans tau t t' -> exists n k x, trans0 t (ChoiceV n k) /\ t' ≅ k x.
+Proof.
+  intros. apply trans_productive in H as (? & ? & ? & ?).
+  inv H0.
+  - rewrite EQ in H1. inv_trans.
+  - rewrite EQ in H1. inv_trans.
+  - rewrite EQ in H1. inv_trans. etrans.
+Qed.
+
+Lemma trans_obs_trans0 {E X Y} : forall (t t' : ctree E X) e (x : Y),
+  trans (obs e x) t t' -> exists k, trans0 t (Vis e k) /\ t' ≅ k x.
+Proof.
+  intros. apply trans_productive in H as (? & ? & ? & ?).
+  inv H0.
+  - rewrite EQ in H1. inv_trans.
+  - rewrite EQ in H1. inv_trans.
+    apply obs_eq_invT in EQl as ?. subst.
+    apply obs_eq_inv in EQl as [<- <-]. etrans.
+  - rewrite EQ in H1. inv_trans.
+Qed.
+
+(* transi *)
+
+Inductive transi {E F X} (h : E ~> ctree F) : @label F -> ctree E X -> ctree E X -> Prop :=
+| transi_val : forall (x : X) t t',
+    trans (val x) t t' ->
+    transi h (val x) t t'
+| transi_tau : forall t t',
+    trans tau t t' ->
+    transi h tau t t'
+| transi_obs : forall Y (e : E Y) x l t t' t'',
+    trans (obs e x) t t' ->
+    t0_det t'' (Ret x) ->
+    trans l (h _ e) t'' ->
+    transi h l t t'
+| transi_obs0 : forall Y (e : E Y) l x t t' t'',
+    trans (obs e x) t t' ->
+    transi h l t' t'' ->
+    trans (val x) (h _ e) CTree.stuckI ->
+    transi h l t t''
+.
+
+Lemma transi_choiceI {E F X} (h : E ~> ctree F) : forall l (t' : ctree E X) n k x,
+  transi h l (k x) t' -> transi h l (ChoiceI n k) t'.
+Proof.
+  intros. inv H.
+  - apply transi_val. etrans.
+  - apply transi_tau. etrans.
+  - eapply transi_obs; etrans.
+  - eapply transi_obs0; etrans.
+Qed.
+
+#[global] Instance transi_equ :
+  forall {E F X} (h : E ~> ctree F) l,
+  Proper (equ eq ==> equ eq ==> flip impl) (@transi E F X h l).
+Proof.
+  cbn. intros.
+  revert x x0 H H0. induction H1; intros.
+  - apply transi_val. rewrite H0, H1. apply H.
+  - apply transi_tau. rewrite H0, H1. apply H.
+  - rewrite <- H2, <- H3 in *. eapply transi_obs; eauto.
+  - rewrite <- H2 in *. eapply transi_obs0; eauto.
+Qed.
+
+#[global] Instance transi_equ' :
+  forall {E F X} (h : E ~> ctree F) l,
+  Proper (equ eq ==> equ eq ==> impl) (@transi E F X h l).
+Proof.
+  cbn. intros. rewrite <- H, <- H0. apply H1.
+Qed.
+
+Lemma trans0_transi {E F X} (h : E ~> ctree F) :
+  forall l (t t' t'' : ctree E X), trans0 t t' -> transi h l t' t'' -> transi h l t t''.
+Proof.
+  intros.
+  red in H. rewrite (ctree_eta t). rewrite (ctree_eta t') in H0.
+  genobs t ot. genobs t' ot'. clear t Heqot. clear t' Heqot'.
+  revert l t'' H0. induction H; intros.
+  - rewrite H. apply H0.
+  - eapply transi_choiceI. setoid_rewrite <- ctree_eta in IHtrans0_. apply IHtrans0_. apply H0.
+Qed.
+
+Lemma transi_sbisim {E F X} (h : E ~> ctree F) :
+  forall l (t t' u : ctree E X), transi h l t t' ->
+  t ~ u ->
+  exists u', transi h l u u' /\ t' ~ u'.
+Proof.
+  intros. revert u H0.
+  induction H; intros.
+  - step in H0. destruct H0 as [? _]. apply H0 in H. destruct H.
+    exists x0. split. now apply transi_val. apply H1.
+  - step in H0. destruct H0 as [? _]. apply H0 in H. destruct H.
+    exists x. split. now apply transi_tau. apply H1.
+  - step in H2. destruct H2 as [? _]. apply H2 in H. destruct H.
+    exists x0. split. eapply transi_obs; eauto. apply H3.
+  - step in H2. destruct H2 as [? _]. apply H2 in H. destruct H.
+    apply IHtransi in H3 as (? & ? & ?). exists x1.
+    split. eapply transi_obs0; eauto. apply H4.
+Qed.
+
+Lemma transi_trans {E F X} (h : E ~> ctree F) (Hh : forall X e, vsimple (h X e)) :
+  forall l (t t' : ctree E X),
+  transi h l t t' -> exists t0, trans l (interp h t) t0 /\ t0_det t0 (interp h t').
+Proof.
+  intros. induction H.
+  - exists CTree.stuckI. apply trans_val_inv in H as ?.
+    apply trans_val_trans0 in H as [].
+    eapply trans0_interp in H. rewrite interp_ret in H. setoid_rewrite H0.
+    setoid_rewrite interp_choice. setoid_rewrite bind_choice. setoid_rewrite choice0_always_stuck.
+    eapply trans0_trans in H; etrans. split; etrans. now left.
+  - exists (TauI (interp h t')). split; [| eright; eauto; now left ].
+    apply trans_tau_trans0 in H as (? & ? & ? & ? & ?).
+    eapply trans0_interp in H. setoid_rewrite H0. eapply trans0_trans; etrans.
+    setoid_rewrite interp_choice. setoid_rewrite bind_choice. setoid_rewrite bind_ret_l.
+    econstructor. reflexivity.
+  - exists (x <- t'';; TauI (interp h t')).
+    split. 2: { eapply t0_det_bind_ret_l; eauto. eright; eauto. now left. }
+    apply trans_obs_trans0 in H as (? & ? & ?).
+    eapply trans0_interp in H. setoid_rewrite H2. eapply trans0_trans; etrans.
+    setoid_rewrite interp_vis.
+    eapply trans_bind_l with (k := fun x => TauI (interp h (x0 x))) in H1.
+    setoid_rewrite t0_det_bind_ret_l_equ in H1 at 2; eauto.
+    { intro. inv H3. apply trans_val_inv in H1. rewrite H1 in H0. inv H0. step in H3. inv H3. step in H4. inv H4. }
+  - destruct IHtransi as (? & ? & ?).
+    destruct (Hh Y e). 2: { destruct H4. rewrite H4 in H1. apply trans_vis_inv in H1 as (? & ? & ?). step in H1. inv H1. }
+    destruct H4. rewrite H4 in H1. inv_trans. subst.
+    exists x0. split. 2: auto.
+    apply trans_obs_trans0 in H as (? & ? & ?). eapply trans0_interp in H.
+    setoid_rewrite interp_vis in H. setoid_rewrite H4 in H. setoid_rewrite bind_ret_l in H.
+    eapply trans0_trans; etrans. setoid_rewrite <- H1. etrans.
+Qed.
+
+(** Various lemmas for the proof that interp preserves sbisim in some cases. *)
+
+Lemma interp_ret_inv {E F X} (h : E ~> ctree F) : forall (t : ctree E X) r,
+  interp h t ≅ Ret r -> t ≅ Ret r.
+Proof.
+  intros. setoid_rewrite (ctree_eta t) in H. setoid_rewrite (ctree_eta t).
+  destruct (observe t) eqn:?.
+  - rewrite interp_ret in H. step in H. inv H. reflexivity.
+  - rewrite interp_vis in H. apply ret_equ_bind in H as (? & ? & ?). step in H0. inv H0.
+  - rewrite interp_choice in H. setoid_rewrite bind_choice in H. step in H. inv H.
+Qed.
+
+Lemma bind_tau_r {E X Y} : forall (t : ctree E X) (k : X -> ctree E Y),
+  x <- t;; TauI (k x) ≅ x <- (x <- t;; TauI (Ret x));; k x.
+Proof.
+  intros. rewrite bind_bind. upto_bind_eq. rewrite bind_tauI. setoid_rewrite bind_ret_l. reflexivity.
+Qed.
+
+Lemma trans_interp_inv_gen {E F X Y} (h : E ~> ctree F) (Hh : forall X e, vsimple (h X e)) :
+  forall l (k : Y -> ctree E X) t' (pre : ctree F Y),
+  is_simple pre ->
+  trans l (x <- pre;; interp h (k x)) t' ->
+  exists t0, t0_det t' (interp h t0) /\
+    ((exists l t1 x, trans l pre t1 /\ t0_det t1 (Ret x) /\ t0 ≅ k x) \/
+    exists x, trans (val x) pre CTree.stuckI /\ trans l (interp h (k x)) t' /\ transi h l (k x) t0).
+Proof.
+  intros * Hpre H.
+  do 3 red in H. remember (observe (x <- pre;; interp h (k x))) as oi.
+  setoid_rewrite (ctree_eta t') at 1.
+  setoid_rewrite (ctree_eta t') at 2.
+  genobs t' ot'. clear t' Heqot'.
+  assert (go oi ≅ x <- pre;; interp h (k x)).
+  { rewrite Heqoi, <- ctree_eta. reflexivity. } clear Heqoi.
+  revert Y k pre Hpre H0. induction H; intros.
+  - (*apply Stepchoice in H as ?.
+    change (ChoiceIF n k) with (observe (ChoiceI n k)) in H1. rewrite H0 in H1.
+       change t with (observe (go t)) in H1. rewrite trans__trans in H1.*)
+    destruct n. now apply Fin.case0.
+    symmetry in H0. apply choice_equ_bind in H0 as ?.
+    destruct H1 as [[] | (? & ? & ?)].
+    + rewrite H1 in H0. rewrite bind_ret_l in H0. setoid_rewrite H1. clear pre Hpre H1.
+      rewrite (ctree_eta (k0 x0)) in H0. destruct (observe (k0 x0)) eqn:?.
+      * rewrite interp_ret in H0. step in H0. inv H0.
+      * rewrite interp_vis in H0. apply choice_equ_bind in H0 as ?. destruct H1 as [[] | (? & ? & ?)].
+        --rewrite H1, bind_ret_l in H0.
+          apply equ_choice_invT in H0 as ?. destruct H2 as [? _]. apply eq_add_S in H2 as <-.
+          simple apply equ_choice_invE with (x := x) in H0.
+          rewrite <- H0 in H.
+          specialize (IHtrans_ _ (fun (_ : unit) => k1 x1) (Ret tt)).
+          edestruct IHtrans_. { apply is_simple_ret. } { rewrite <- ctree_eta, bind_ret_l, H0. reflexivity. }
+          destruct H2. exists x2. split; auto. right. destruct H3.
+          { destruct H3 as (? & ? & ? & ? & ? & ?). inv_trans. subst.
+            inv H4. step in H3. inv H3. step in H6. inv H6. }
+          destruct H3 as (_ & _ & ? & ?). exists x0. split. etrans. split.
+          ++setoid_rewrite (ctree_eta (k0 x0)). rewrite Heqc.
+            setoid_rewrite interp_vis. setoid_rewrite H1. setoid_rewrite bind_ret_l. apply trans_tauI. apply H3.
+          ++setoid_rewrite (ctree_eta (k0 x0)). rewrite Heqc.
+            eapply transi_obs0; etrans. rewrite H1. etrans.
+        --destruct (Hh X0 e).
+          destruct H3. rewrite H3 in H1. step in H1. inv H1.
+          destruct H3. rewrite H3 in H1. step in H1. inv H1.
+          (*specialize (IHtrans_ _ k1 (x <- x1 x;; TauI (Ret x))).
+          edestruct IHtrans_ as (? & ? & ?). { facile admit. }
+          { rewrite <- ctree_eta, bind_bind. setoid_rewrite bind_tauI. setoid_rewrite bind_ret_l. apply H2. }
+          destruct H4. admit.
+          exists x2. split; auto. right. exists x0. split; etrans.
+          destruct H4 as (? & ? & ? & ?).
+          setoid_rewrite (ctree_eta (k0 x0)). setoid_rewrite Heqc. setoid_rewrite interp_vis. split.
+          eapply trans_bind_r; etrans. rewrite H1.
+          eapply trans_choiceI with (x := x). 2: reflexivity.
+          apply trans_bind_inv in H4 as [].
+          { destruct H4. exfalso. apply H4. constructor. }
+          destruct H4 as (? & ? & ? & ?). inv_trans. subst. etrans.
+          eapply transi_obs0; eauto. rewrite H1. admit.*)
+      * rewrite interp_choice in H0. setoid_rewrite bind_choice in H0. setoid_rewrite bind_ret_l in H0.
+        apply equ_choice_invT in H0 as ?. destruct H1 as [-> ->].
+        simple apply equ_choice_invE with (x := x) in H0 as ?.
+        specialize (IHtrans_ _ (fun _ : unit => k1 x) (TauI (Ret tt))).
+        edestruct IHtrans_ as (? & ? & ?).
+        { apply is_simple_tauI_ret. }
+        { rewrite <- ctree_eta. setoid_rewrite bind_choice. setoid_rewrite bind_ret_l. now rewrite H1. }
+        destruct H3.
+        { destruct H3 as (? & ? & ? & ? & ? & ?). inv_trans. subst.
+          inv H4. step in H3. inv H3. step in H5. inv H5. }
+        destruct H3 as (? & ? & ? & ?).
+        exists x1. split; auto. right. exists x0. split; etrans. split.
+        rewrite (ctree_eta (k0 x0)), Heqc, interp_choice. setoid_rewrite bind_choice. setoid_rewrite bind_ret_l.
+        eapply trans_choiceI. 2: reflexivity. apply trans_tauI. apply H4.
+        rewrite (ctree_eta (k0 x0)), Heqc. eapply transi_choiceI; etrans.
+    + specialize (IHtrans_ _ k0 (x0 x)).
+      edestruct IHtrans_ as (? & ? & ?).
+      { apply is_simple_choiceI. red. setoid_rewrite <- H1. apply Hpre. }
+      rewrite <- ctree_eta. apply H2. destruct H4 as [(? & ? & ? & ? & ? & ?) | (? & ? & ? & ?)].
+      * (*setoid_rewrite H5 in H3. clear x1 H5.*)
+        exists (k0 x4). split. { now rewrite H6 in H3. }
+        left. eapply trans_choiceI in H4. 2: reflexivity. rewrite <- H1 in H4. eauto 6.
+      * exists x1. split; auto. right. exists x2. rewrite H1. etrans.
+  - destruct n. now apply Fin.case0.
+    symmetry in H0. apply choice_equ_bind in H0 as ?. destruct H1 as [[] | (? & ? & ?)].
+    + rewrite H1 in H0. rewrite bind_ret_l in H0.
+      rewrite (ctree_eta (k0 x0)) in H0. destruct (observe (k0 x0)) eqn:?.
+      * rewrite interp_ret in H0. step in H0. inv H0.
+      * rewrite interp_vis in H0. apply choice_equ_bind in H0 as ?.
+        destruct H2 as [[] | (? & ? & ?)].
+        { rewrite H2, bind_ret_l in H0. step in H0. inv H0. }
+        pose proof (trans_choiceV x1 x). rewrite <- H2 in H4.
+        edestruct Hh. { destruct H5. rewrite H5 in H4. inv_trans. }
+        destruct H5. rewrite H5 in H4. apply trans_vis_inv in H4 as (? & ? & ?). discriminate.
+        (*--specialize (H3 x).
+          (*rewrite H4 in H3. rewrite bind_ret_l in H3.*)
+          exists (k1 x2).
+          rewrite H in H3. split; auto. rewrite H3, <- ctree_eta.
+          eapply t0_det_bind_ret_l; eauto. eapply t0_det_tau; eauto. constructor; auto.
+          right. exists x0. rewrite H1. split; etrans.
+          setoid_rewrite (ctree_eta (k0 x0)). setoid_rewrite Heqc. split.
+          { setoid_rewrite interp_vis. setoid_rewrite H2. setoid_rewrite bind_choice.
+            econstructor. rewrite <- ctree_eta, H3. reflexivity. }
+          eapply transi_vis; eauto. rewrite H2. etrans.*)
+      * rewrite interp_choice in H0. setoid_rewrite bind_choice in H0.
+        apply equ_choice_invT in H0 as ?. destruct H2 as [-> ->].
+        simple eapply equ_choice_invE in H0 as ?. rewrite bind_ret_l in H2. rewrite H in H2.
+        exists (k1 x). symmetry in H2. split.
+        { rewrite <- ctree_eta. rewrite H2. eapply t0_det_tau; auto. apply t0_det_id; auto. }
+        right. exists x0. rewrite H1. split; etrans.
+        setoid_rewrite (ctree_eta (k0 x0)). setoid_rewrite Heqc. split.
+        { setoid_rewrite interp_choice. rewrite H2. setoid_rewrite bind_choice. setoid_rewrite bind_ret_l.
+          econstructor. now rewrite <- ctree_eta. }
+        econstructor; etrans.
+    + pose proof (trans_choiceV x0 x).
+      rewrite <- H1 in H3. edestruct Hpre.
+      { apply H4 in H3. inv H3. }
+      apply H4 in H3 as [].
+      specialize (H2 x).
+      (*rewrite H3, bind_ret_l in H2.*)
+      exists (k0 x1). rewrite H in H2. split. { rewrite <- ctree_eta, H2. eapply t0_det_bind_ret_l; eauto. now left. }
+      left. exists tau, (x0 x), x1. split; auto. rewrite H1. etrans.
+  - symmetry in H0. apply vis_equ_bind in H0 as ?. destruct H1 as [[] | (? & ? & ?)].
+    + rewrite H1 in H0. rewrite bind_ret_l in H0.
+     rewrite (ctree_eta (k0 x0)) in H0. destruct (observe (k0 x0)) eqn:?.
+      * rewrite interp_ret in H0. step in H0. inv H0.
+      * rewrite interp_vis in H0. apply vis_equ_bind in H0 as ?.
+        destruct H2 as [[] | (? & ? & ?)].
+        { rewrite H2, bind_ret_l in H0. step in H0. inv H0. }
+        pose proof (trans_vis e x x1). rewrite <- H2 in H4.
+        edestruct Hh. { destruct H5. rewrite H5 in H4. inv H4. }
+        destruct H5. rewrite H5 in H4. (*destruct H4 as [? ?].*)
+        specialize (H3 x). rewrite H5 in H2.
+        apply equ_vis_invT in H2 as ?. subst.
+        apply equ_vis_invE in H2 as ?. destruct H6 as [-> ?].
+        rewrite <- H6 in *. rewrite bind_ret_l in H3.
+        exists (k1 x).
+        rewrite H in H3. split. { rewrite <- ctree_eta, H3. eright; eauto. eleft; auto. }
+        right.
+        exists x0. rewrite H1. split; etrans.
+        setoid_rewrite (ctree_eta (k0 x0)). setoid_rewrite Heqc. split.
+        { setoid_rewrite interp_vis. rewrite H5. setoid_rewrite bind_vis.
+          econstructor. rewrite bind_ret_l. rewrite <- H3, <- ctree_eta. reflexivity. }
+        eapply transi_obs; etrans. 2: { rewrite H5. etrans. } now left.
+      * rewrite interp_choice in H0. setoid_rewrite bind_choice in H0.
+        step in H0. inv H0.
+    + pose proof (trans_vis e x x0).
+      rewrite <- H1 in H3. edestruct Hpre.
+      { apply H4 in H3. inv H3. }
+      apply H4 in H3 as [].
+      specialize (H2 x).
+      exists (k0 x1). rewrite H in H2. split.
+      { rewrite <- ctree_eta, H2. eapply t0_det_bind_ret_l; eauto. now left. }
+      left. exists (obs e x), (x0 x), x1. split; auto. rewrite H1. etrans.
+     - exists (CTree.stuckI). split.
+       + left.
+         setoid_rewrite interp_choice. setoid_rewrite bind_choice. rewrite !choice0_always_stuck. reflexivity.
+       + right. symmetry in H0. apply ret_equ_bind in H0 as (? & ? & ?).
+         exists x. rewrite H. split; etrans. split.
+         rewrite H0. rewrite choice0_always_stuck. etrans.
+         apply interp_ret_inv in H0. rewrite H0. constructor; etrans.
+Qed.
+
+Lemma trans_interp_inv {E F X} (h : E ~> ctree F) (Hh : forall X e, vsimple (h X e)) :
+  forall l (t : ctree E X) t',
+  trans l (interp h t) t' ->
+  exists l t0, t0_det t' (interp h t0) /\ transi h l t t0.
+Proof.
+  intros.
+   assert (trans l (TauI (Ret tt);; interp h t) t').
+   { etrans. }
+  eapply trans_interp_inv_gen in H0; eauto. destruct H0 as (? & ? & ?).
+  destruct H1 as [(? & ? & ? & ? & ? & ?) | (? & ? & ? & ?)].
+  - inv_trans. subst. inv H2. step in H1. inv H1. step in H3. inv H3.
+  - inv_trans. subst. eauto.
+  - left. intros. inv_trans. subst. constructor.
+Qed.
+
+(** The main theorem stating that interp preserves sbisim. *)
+
+Theorem interp_sbisim_gen {E F X Y} (h : E ~> ctree F) (Hh : forall X e, vsimple (h X e)) :
+  forall (k k' : X -> ctree E Y) (pre pre' : ctree F X),
+  (forall x, sbisim (k x) (k' x)) ->
+  pre ≅ pre' ->
+  vsimple pre ->
+  sbisim (a <- pre;; TauI (interp h (k a))) (a <- pre';; TauI (interp h (k' a))).
+Proof.
+  revert X. coinduction R CH.
+  symmetric using idtac.
+  { intros. apply H; eauto.  intros. rewrite H0. reflexivity. now rewrite H1. red; now setoid_rewrite <- H1. }
+  assert (CH' : forall (t t' : ctree E Y), t ~ t' -> st R (interp h t) (interp h t')).
+  {
+    intros.
+    assert (st R (a <- Ret tt;; TauI (interp h ((fun _ => t) a)))
+      (a <- Ret tt;; TauI (interp h ((fun _ => t') a)))).
+    { apply CH; eauto. left; eauto. }
+    rewrite !bind_ret_l in H0.
+    rewrite !sb_tauI in H0.
+    apply H0.
+  }
+  intros. setoid_rewrite <- H0. clear pre' H0. cbn. intros.
+  copy H0. rewrite bind_tau_r in H0.
+  eapply trans_interp_inv_gen in H0 as (? & ? & ?); auto.
+  2: { destruct H1 as [[] | []]; rewrite H1.
+    rewrite bind_ret_l. apply is_simple_tauI_ret.
+    rewrite bind_trigger. right. intros. inv_trans. subst.
+    exists x0. rewrite EQ. eright. left. reflexivity. reflexivity.
+  }
+  destruct H2.
+  - destruct H2 as (? & ? & ? & ? & ? & ?). rewrite H4 in H0. clear x H4.
+    destruct H1 as [[] | []].
+    + rewrite H1, bind_ret_l in H2. rewrite H1, bind_ret_l in cpy. inv_trans. subst.
+      inv H3. step in H2. inv H2. step in H4. inv H4.
+    + rewrite H1 in *. rewrite bind_trigger in H2. apply trans_vis_inv in H2 as (? & ? & ?). subst.
+      (* todo lemma *)
+      rewrite H2 in H3. inv H3. step in H4. inv H4.
+      apply equ_choice_invE in H5. 2: apply Fin.F1.
+      rewrite <- H5 in H4. inv H4. 2: { step in H6. inv H6. }
+      step in H3. inv H3. clear x1 H2 t H5.
+      rewrite bind_trigger in cpy. apply trans_vis_inv in cpy. destruct cpy as (? & ? & ?). subst.
+      exists (TauI (interp h (k' x0))). rewrite H1. rewrite bind_trigger. now constructor.
+      rewrite H2, !sb_tauI. apply CH'. apply H.
+  - destruct H2 as (? & ? & ? & ?).
+    destruct H1 as [[] | []]. 2: { rewrite H1 in H2. setoid_rewrite bind_trigger in H2. inv_trans. }
+    rewrite H1 in *. rewrite bind_ret_l in H2. inv_trans. subst. clear EQ.
+    eapply transi_sbisim in H4; eauto. destruct H4 as (? & ? & ?).
+    apply transi_trans in H2 as (? & ? & ?); auto.
+    exists x2. rewrite H1, bind_ret_l. etrans.
+    assert (st R (interp h x) (interp h x0)).
+    { apply CH'. apply H4. }
+    rewrite sbisim_t0_det. 2: apply H0.
+    setoid_rewrite sbisim_t0_det at 3. 2: apply H5.
+    apply H6.
+Qed.
+
+#[global] Instance interp_sbisim {E F R} (h : E ~> ctree F) (Hh : forall X e, vsimple (h X e)) :
+  Proper (sbisim ==> sbisim) (interp h (T := R)).
+Proof.
+  cbn. intros.
+  assert (a <- Ret tt;; TauI (interp h ((fun _ => x) a)) ~
+    a <- Ret tt;; TauI (interp h ((fun _ => y) a))).
+  apply interp_sbisim_gen; auto.
+  red; eauto.
+  rewrite !bind_ret_l, !sb_tauI in H0. apply H0.
+Qed.
+
 (*
 Lemma interp_trigger {E F : Type -> Type} {R : Type}
       (f : E ~> (itree F))
@@ -143,4 +810,3 @@ Proof.
   reflexivity.
 Qed.
 *)
-
